Date: 08-**CHANGE THIS**-2023

## Raw Notes

- To derive the power rule for natural numbers, we can use the binomial theorem on the limit definition:
	- We first write the limit and expand the $(x+h)^n$ term with the binomial theorem (where ${n\choose i}$ is $\text{nCi}$ and the last step is valid because the first term of the sum is $x^n$): $$\lim _{h\to 0}\frac{\left(x+h\right)^n-x^n}{h}=\lim _{h\to 0}\frac{\sum _{i=0}^n\binom{n}{i}x^{n-i}h^i-x^n}{h}=\lim _{h\to 0}\frac{\sum _{i=1}^n\binom{n}{i}x^{n-i}h^i}{h}$$
	- We can now factor out the $h$, and notice that $h^{i-1}$ is always 0 except when $i-1$ is 0 (then, remember that the $h$ cancels out and that $h^{i-1}$ is just 1): $$\lim _{h\to 0}\sum _{i=1}^n\binom{n}{i}x^{n-i}h^{i-1}=\binom{n}{1}x^{n-1}=nx^{n-1}$$
	- Therefore, the derivative of $x^n$ is $nx^{n-1}$.
	- The rule extends to $n\in\mathbb{R}$.
	- For example, $\left(x^3\right)'=3x^2$, and $\left(\sqrt{x}\right)'=\left(x^{\frac{1}{2}}\right)'=\frac{1}{2}x^{-\frac{1}{2}}=\frac{1}{2x^{\frac{1}{2}}}=\frac{1}{2\sqrt x}$ 
- When using the power rule, it is important to be cautious when subtracting one from the exponent, especially when dealing with rational and negative exponents.
- It isn't really necessary to rationalize the negative exponent for the FRQs, but for MCQs, answers will usually be rationalized so it will be easier for you to compare answers.

## Key Takeaways



## Questions

