Date: October 2023

## Raw Notes

- The functions we have seen so far were in the form $y=f(x)$. Sometimes we have to differentiate something in the form of $f(x,y)=g(x,y)$ however, for example, $x^2+y^2=2x(x+y)$.
- We can do something called implicit differentiation. It works kind of like this: you assume $y$ is a function of $x$, and when differentiating $y$ with respect to $x$, you treat it regularly but tack on a $\frac{dy}{dx}$ at the end. For example: $$\frac{d}{dx}y^3=3y^2\cdot\frac{dy}{dx}$$
- We multiply the $\frac{dy}{dx}$ as a result of the chain rule. In particular, let's say $u=y, u'=y', f(u)=u^3, f'(u)=3u^2$. Then, applying the chain rule, we get the above equation, noting that $y'=\frac{dy}{dx}$.
- Now, if a question asks to solve for $\frac{dy}{dx}$, you should first implicitly differentiate, then group all the terms with and without $\frac{dy}{dx}$ respectively, and solve. For example, to solve for $\frac{dy}{dx}$ in $2x^2-x^2y+y^4=24$, we first implicitly differentiate: $$2x^2-x^2y+y^4=24\ \Rightarrow \ 4x-\left(2xy+x^2\cdot \frac{dy}{dx}\right)+4y^3\cdot \frac{dy}{dx}=0$$
- We then simplify and group all terms: $$\ 4x-2xy-x^2\frac{dy}{dx}+4y^3\frac{dy}{dx}=0\ \Rightarrow \ \frac{dy}{dx}\left(4y^3-x^2\right)=2xy-4x$$
- Then, divide both sides by $4y^3-x^2$ to isolate $\frac{dy}{dx}$: $$\ \frac{dy}{dx}\frac{4y^3-x^2}{4y^3-x^2}=\frac{2xy-4x}{4y^3-x^2}\ \Rightarrow \ \frac{dy}{dx}=\frac{2xy-4x}{4y^3-x^2}$$
- To implicitly differentiate at a point, differentiate with respect to $x$, substitute the known $x$ and $y$ values of the point, and solve for $\frac{dy}{dx}$. For example, to determine the tangent line to the curve $3x^3+7y^3=10y$ at $(1,1)$, we first implicitly differentiate with respect to $x$: $$3x^3+7y^3=10y\Rightarrow 9x^2+21y^2\frac{dy}{dx}=10\frac{dy}{dx}$$
- We can then isolate $\frac{dy}{dx}$: $$\frac{dy}{dx}(10-21y^2)=9x^2\Rightarrow \frac{dy}{dx}=\frac{9x^2}{10-21y^2}$$
- Then, we can solve for the slope of the curve at $(1,1)$ by plugging in $x$ and $y$: $$\frac{dy}{dx}\Big|_{x,y=1,1}=\frac{9(1)^2}{10-21(1)}=-\frac{9}{11}$$
- Then, we can use the equation of a line given a slope and a point and we are done: $$y-1=-\frac{9}{11}(x-1)$$
## Key Takeaways

The derivative of $y$ with respect to x is is $\frac{dy}{dx}$. Here is an example of how to differentiate with respect to $x$: $$\frac{d}{dx}(2x^3+3y^4)=6x^2+12y^3\cdot \frac{dy}{dx}$$

## Questions

